Progress BoundVars

src/Util/List.v
@@ -1,10 +1,11 @@
-Require Import Coq.Lists.List.
-Require Import Coq.Strings.String.
-Import ListNotations.
+From Coq Require Import 
+  Lists.List
+  Strings.String.
 
-Local Open Scope list_scope.
+Import ListNotations.
 Local Open Scope string_scope.
 
+From QuickChick Require Import QuickChick.
 
 Fixpoint lookup {X:Type} (k : string) (l : list (string * X)) : option X :=
   match l with
@@ -18,13 +19,31 @@ Inductive Lookup {A B :Type} (k : A) (v : B) : list (A * B) -> Prop :=
 .
 
 Lemma Lookup_lookup : forall A k (v : A) kvs, Lookup k v kvs <-> lookup k kvs = Some v.
-Admitted.
+Proof.
+  intros. generalize dependent k. generalize dependent v.
+  induction kvs; split; intros; simpl; inversion H.
+    - rewrite eqb_refl. reflexivity.
+    - rewrite eqb_sym. apply (eqb_neq k k') in H2. rewrite H2. apply IHkvs. apply H3.
+    - destruct a as [k' v']. destruct (k' =? k) eqn:E.
+      + apply eqb_eq in E. inversion H1. subst. apply Here.
+      + apply There. 
+        * rewrite eqb_sym in E. apply eqb_neq in E. apply E.
+        * apply IHkvs in H1. apply H1.
+Qed.
 
 Lemma Lookup_functional : forall A B (k : A) (v v' : B) kvs,  Lookup k v kvs -> Lookup k v' kvs -> v = v'.
-Admitted.
+Proof. 
+  induction kvs; intros; inversion H.
+    - subst. inversion H0.
+      + reflexivity.
+      + exfalso. apply H3. reflexivity.
+    - subst. inversion H0.
+      + apply H3 in H2. inversion H2.
+      + apply IHkvs. apply H4. apply H7.
+Qed.
 
 Lemma Lookup_unique : forall A B (k : A) (v : B) kvs (P P' : Lookup k v kvs), P = P'.
-Admitted.
+Admitted. 
 
 Lemma Lookup_In : forall A B (k : A) (v : B) kvs, NoDup kvs -> In (k, v) kvs <-> Lookup k v kvs.
 Admitted.
@@ -49,9 +68,29 @@ Definition forall2b {A} (p : A -> A -> bool) := fix f xs ys :=
     | _        , _         => false
   end.
 
-
-
-
 Lemma mdrop_nil : forall X ns,
     @mdrop X ns nil = nil.
 Proof. induction ns; auto. Qed.
+
+
+Inductive In {A : Type} (x : A) : list A -> Prop :=
+  | In_Here  : forall {xs}, In  x (x :: xs)
+  | In_There : forall {x' xs}, In  x xs -> In x (x' :: xs).
+
+Lemma In_Coq_In_equal : forall A (x : A) xs, In x xs <-> Coq.Lists.List.In x xs.
+Proof.
+  intros. generalize dependent x. induction xs; split; intros; simpl; inversion H.
+    - left. reflexivity.
+    - right. apply IHxs. apply H1.
+    - subst. apply In_Here.
+    - apply In_There. apply IHxs. apply H0.
+Qed.
+
+Derive DecOpt for (In x xs).
+
+(** TODO: doesnt work?
+Instance In_DecOpt_sound x xs : DecOptSoundPos (In x xs).
+Proof. derive_sound. Qed.
+ *)
+
+
